src/tls/Model.CRF.fst
@@ -1,0 +1,103 @@
+﻿(** computational assumption: collision resistance *)
+module Model.CRF
+
+/// This module should not be extracted 
+
+open EverCrypt.Hash // only for the specs (renamings)
+
+//2018.04.24 SZ: to be moved elsewhere, set to false for real extraction
+//inline_for_extraction
+// let crf _ = false
+assume val crf: alg -> Tot bool
+
+let h = Spec.Hash.hash 
+
+(* Depending on a single, global idealization function, we keep a global
+    inverse table for all (finalized) hash computations, and we use it to
+    detect concrete collisions. Technically, this is modelled as
+    non-termination of a stateful, partially-correct finalize filter.
+    This may depend on some prior flag to keep the hashed input in the
+    incremental hash implementation. (This is always the case for now.)  *)
+
+open Mem 
+module MDM = FStar.Monotonic.DependentMap 
+
+type hashable (a:alg) = v:Seq.seq UInt8.t {Seq.length v < maxLength a}
+// the precise types guarantee that the table stays empty when crf _ = false
+private type range = | Computed: a: alg {crf a} -> t: tag a -> range
+private type domain (r:range) =
+  b:Seq.seq UInt8.t {
+    let Computed a t = r in 
+    Seq.length b < maxLength a /\ 
+    h a b = t}
+
+private let inv (f:MDM.partial_dependent_map range domain) = True // a bit overkill?
+private let table : MDM.t tls_tables_region range domain inv = MDM.alloc()
+
+// witnessing that we hashed this particular content (for collision detection)
+// to be replaced by a witness of inclusion in a global table of all hash computations.
+// (not sure how to manage that table)
+
+//val hashed: a:alg -> b:bytes -> Type
+abstract type hashed (a:alg) (b:hashable a) =
+  crf a ==> (
+    let t = h a b in
+    witnessed (MDM.contains table (Computed a t) (b <: domain (Computed a t))))
+
+val crf_injective (a:alg) (b0 b1:hashable a): ST unit  // should be STTot
+  (requires fun h0 -> hashed a b0 /\ hashed a b1)
+  (ensures fun h0 _ h1 -> h0 == h1 /\ (crf a /\ h a b0 == h a b1 ==> b0 == b1))
+let crf_injective a b0 b1 =
+  if crf a then (
+    recall table;
+    let f = !table in
+    testify(MDM.contains table (Computed a (h a b0)) b0);
+    testify(MDM.contains table (Computed a (h a b1)) b1)
+  )
+
+/// We use [stop] to model the exclusion of "bad" events, in this case
+/// a hash collision.  We should review this "flagless" style for
+/// crypto modelling.
+
+noextract 
+private val stop: s:string -> Stack 'a
+  (requires fun h -> True)
+  (ensures fun h0 r h1 -> False)
+let rec stop (s:string) = stop s
+
+val hash: a:alg -> v:hashable a -> Stack (tag a)
+  (requires fun h0 -> True)
+  (ensures fun h0 t h1 ->
+    LowStar.Buffer.(modifies loc_none h0 h1) /\
+    t == h a v /\ 
+    hashed a v
+  )
+
+open LowStar.Buffer
+
+module ST = FStar.HyperStack.ST 
+
+let hash a v =
+  let h0 = ST.get() in 
+  let t = Spec.Hash.hash a v in 
+  if crf a then (
+    let x = Computed a t in
+    match MDM.lookup table x with
+      | None -> MDM.extend table x v
+      | Some v' -> if v <> v' then stop "hash collision detected");
+  let h1 = ST.get() in 
+  //19-05-25 TODO stuck with an old library
+  assume(h0 == h1); //modifies loc_none h0 h1);
+  t
+
+#set-options "--z3rlimit 100"
+// sanity check
+
+open FStar.Seq
+private val test (a:alg {crf a}) (b0 b1: hashable a): St unit
+let test a b0 b1 =
+  let t0 = hash a b0 in 
+  let t1 = hash a b1 in
+  crf_injective a b0 b1;
+  if t0 = t1 then assert(b0 == b1)
+  
