src/tls/Old.KeySchedule.fst
@@ -9,13 +9,14 @@ open FStar.Error
 //open FStar.Integers 
 
 open TLSError
+open TLS.Callbacks
 open TLSConstants
 open Extensions
 open TLSInfo
 open Range
 open StatefulLHAE
 open HKDF
-open PSK
+//open PSK
 
 module MDM = FStar.Monotonic.DependentMap
 module HS = FStar.HyperStack
