src/tls/TC.fst
@@ -1,0 +1,76 @@
+module TC 
+
+open FStar.Preorder
+open FStar.Tactics
+
+noeq
+type closure (#a:Type0) (r:relation a) : a -> a -> Type0 =
+| Refl: x:a -> closure r x x
+| Step: x:a -> y:a -> r x y -> closure r x y
+| Closure: x:a -> y:a -> z:a -> closure r x y -> closure r y z -> closure r x z
+
+val closure_reflexive: #a:Type0 -> r:relation a -> Lemma (reflexive (closure r))
+let closure_reflexive #a r =
+  assert (forall x. closure r x x) by
+    (let x = forall_intro () in mapply (quote Refl))
+
+val closure_transitive: #a:Type0 -> r:relation a -> Lemma (transitive (closure r))
+let closure_transitive #a r =
+  assert (transitive (closure r)) by
+    (let x = forall_intro () in
+     let y = forall_intro () in
+     let z = forall_intro () in
+     let h = implies_intro () in
+     and_elim (binder_to_term h);
+     let h1 = implies_intro () in
+     let h2 = implies_intro () in
+     mapply (quote (Closure #a #r));
+     assumption ();
+     assumption ())
+
+val reflexive_transitive_closure: #a:Type0 -> relation a -> preorder a
+let reflexive_transitive_closure #a r =
+  closure_reflexive r;
+  closure_transitive r;
+  closure r
+
+// anticipating abstraction 
+let step #a #r (x y:a) (#h: r x y): closure r x y = Step x y h
+
+assume val inv_closure:
+  #a: Type0 -> 
+  step: relation a ->
+  p: (a -> Type0) -> 
+  hr: (x:a -> y:a {p x /\ step x y} -> Lemma(p y)) ->
+  x: a -> y: a {p x /\ closure step x y} -> Lemma(p y)
+
+// test 
+type state = 
+  | A 
+  | B 
+  | C 
+let r x y = 
+  match x, y with 
+  | A, B
+  | B, C
+  | C, B -> True
+  | _ -> False
+let cl = reflexive_transitive_closure r
+let p = function | A -> False | B | C -> True 
+let q = function | A | B -> False | C -> True 
+
+let hp (x:state) (y:state{p x /\ r x y}): Lemma(p y) = ()
+// match x, y with 
+// | B, C -> assert(p y)
+// | C, B -> assert(p y)
+
+// let hq x y: Lemma(q x /\ r x y ==> q y) = ()
+
+let test = inv_closure r p hp 
+
+let f (x:state{ cl B x }) = 
+  test B x;
+  assert(x <> A)
+
+
+
