src/tls/TLS.Callbacks.fsti
@@ -1,0 +1,240 @@
+module TLS.Callbacks
+
+open FStar.Bytes
+open Mem 
+
+//include Parsers.ProtocolVersion 
+include Parsers.ServerName
+include Parsers.ProtocolName
+include Parsers.ProtocolNameList
+include Parsers.PskIdentity
+include CipherSuite 
+
+/// opaque context pointers provided by the application and passed back to it.
+
+val context: Type0
+val default_context: unit -> EXT context 
+
+/// ------------------------------------------------------------------------------
+/// Ticket callback, used to store received tickets with their authenticated info
+
+type psk_identifier = pskIdentity_identity
+
+[@unifier_hint_injective]
+inline_for_extraction
+let vlbytespl (min max: nat) = (x: bytes { min <= length x /\ length x <= max })
+
+type pskInfo = {
+  ticket_nonce: option (vlbytespl 0 255);
+  time_created: UInt32.t;
+  ticket_age_add: UInt32.t;
+  allow_early_data: bool;      // New draft 13 flag
+  allow_dhe_resumption: bool;  // New draft 13 flag
+  allow_psk_resumption: bool;  // New draft 13 flag
+  early_ae: aeadAlg;
+  early_hash: hash_alg;
+  identities: bytes * bytes; // TODO certs 
+}
+
+type ticketInfo =
+  | TicketInfo_12 of Parsers.ProtocolVersion.protocolVersion * cipherSuite * ems:bool
+  | TicketInfo_13 of pskInfo
+
+type ticket_seal = b:bytes{length b < 65536}
+
+
+/// Calls Client to store received tickets and their context.
+///
+/// TODO consider adding pre-condition capturing the authenticated
+/// properties of the context.
+
+// 2018.03.10 SZ: Allow it to modify [psk_region]?
+// Missing refinements on arguments from types in PSK
+
+inline_for_extraction
+type ticket_cb_fun =
+  sni:string -> 
+  ticket:ticket_seal -> 
+  info:ticketInfo -> 
+  rawkey:bytes -> 
+  ST unit
+    (requires fun _ -> True)
+    (ensures fun h0 _ h1 -> modifies_none h0 h1)
+
+noeq type ticket_cb = {
+  ticket_context: context;
+  new_ticket: context -> ticket_cb_fun;
+}
+
+
+/// ------------------------------------------------------------------------------
+/// Negotiation callback, for both clients and servers.
+///
+/// Only the server gets to retry or to respond with
+/// custom_extensions. Consider separating the two callbacks.
+
+/// Custom Extensions sent and received from the negotiation callback.
+
+include Parsers.ExtensionType
+include Parsers.UnknownExtension
+
+// 18-12-22 TODO use a vl wire format instead of a list
+type custom_id = v:UInt16.t{~(known_extensionType_repr v)}
+type custom_extension = custom_id * unknownExtension
+type custom_extensions = list custom_extension
+
+(* Helper functions for the C API to construct the list from array *)
+let empty_custom_extensions () : list custom_extension = []
+let add_custom_extension 
+  (l:list custom_extension) 
+  (hd:custom_id) 
+  (b:bytes {length b < 65533}) = (hd, b) :: l
+
+type cookie = Parsers.Cookie.cookie 
+type nego_action =
+  | Nego_abort: nego_action
+  | Nego_retry: cookie_extra: cookie -> nego_action
+  | Nego_accept: extra_ext: custom_extensions -> nego_action
+
+/// Witnessing the callback's decision as an abstract property that
+/// can be provably authenticated by the peer connection.
+///
+/// This suggests we are not passing enough of the mode, including at
+/// least some unique identifiers. And also that we need to separate
+/// client and server callbacks.
+
+val negotiated:  
+  Parsers.ProtocolVersion.protocolVersion -> 
+  client_ext: bytes -> 
+  cookie: option cookie -> 
+  nego_action -> 
+  Type0
+
+inline_for_extraction 
+type nego_cb_fun =
+  pv: Parsers.ProtocolVersion.protocolVersion -> 
+  client_ext: bytes -> 
+  cookie: option cookie -> 
+  ST nego_action
+    (requires fun _ -> True)
+    (ensures fun h0 r h1 -> 
+      negotiated pv client_ext cookie r /\ 
+      (Nego_retry? r ==> None? cookie /\ modifies_none h0 h1))
+
+noeq type nego_cb = {
+  nego_context: context;
+  negotiate: context -> nego_cb_fun;
+}
+
+// TODO authentication properties: 
+//
+// * cookie: from the retry to the second ClientHello
+// * extensions: from Client to Server, from Server to Client
+
+/// ------------------------------------------------------------------------------
+/// Certificate callbacks
+///
+/// Each callback takes an application context (app_context) and a
+/// function pointer to an application-provided functionality.
+///
+/// The callback is actually performed in FFI.fst, which calls into
+/// ffi.c and takes care of marshalling miTLS parameters like
+/// signatureSchemeList to the types expected by the application.
+///
+/// This explicit representation of closures is necessary for
+/// compiling this to C via KreMLin. The representation is hidden from
+/// callers and the wrappers are provided below to implement it.
+
+type cert_repr = b:bytes {length b < 16777216}
+type cert_type = FFICallbacks.callbacks
+
+include Parsers.SignatureScheme
+include Parsers.SignatureSchemeList
+
+// outline authorization predicates--but we miss identifiers. 
+
+// TODO: parametricity in a "logical payload" formula defined by the
+// handshake, passed as an input to select, used in the preconditiong
+// of sign, and in the postcondition of verify.
+//
+noextract val payload: cert_type -> bytes -> Type0 
+
+noextract 
+val cert_selected: 
+  Parsers.ProtocolVersion.protocolVersion -> 
+  bytes -> 
+  bytes -> 
+  signatureSchemeList -> 
+  cert_type -> 
+  signatureScheme ->
+  Type0 
+inline_for_extraction
+type cert_select_cb_fun = 
+  pv:Parsers.ProtocolVersion.protocolVersion -> 
+  sni:bytes -> 
+  alpn:bytes -> 
+  sig:signatureSchemeList -> 
+  ST (option (cert_type * signatureScheme))
+    (requires fun _ -> True)
+    (ensures fun h0 r h1 -> 
+      modifies_none h0 h1 /\ (
+      match r with 
+      | Some (ct, sa) -> cert_selected pv sni alpn sig ct sa 
+      | None -> True
+      // TODO the caller needs to know the cert_type is for its payload
+      ))
+
+noextract 
+val cert_format: cert_type -> list cert_repr 
+
+noextract 
+val cert_parse: cc: list cert_repr -> option (ct:cert_type{ cc == cert_format ct })
+
+
+// TODO add an error case; use it as default. 
+inline_for_extraction
+type cert_format_cb_fun =
+  ct:cert_type -> 
+  ST (list cert_repr)
+    (requires fun _ -> True)
+    (ensures fun h0 r h1 -> 
+      (r == [] \/ r == cert_format ct) /\
+      modifies_none h0 h1)
+
+inline_for_extraction
+type cert_sign_cb_fun = 
+  ct:cert_type -> 
+  signatureScheme -> 
+  tbs:bytes -> 
+  ST (option bytes)
+    (requires fun _ -> payload ct tbs)
+    (ensures fun h0 _ h1 -> 
+      modifies_none h0 h1)
+
+inline_for_extraction
+type cert_verify_cb_fun = 
+  cc:list cert_repr -> 
+  signatureScheme -> 
+  tbs:bytes -> 
+  sigv:bytes -> ST bool
+    (requires fun _ -> True)
+    (ensures fun h0 b h1 -> 
+      modifies_none h0 h1 /\
+      (b ==> (
+        match cert_parse cc with 
+        | None -> False
+        | Some ct -> payload ct tbs)))
+
+val cert_cb: Type0
+val cert_select_cb: cert_cb -> cert_select_cb_fun
+val cert_format_cb: cert_cb -> cert_format_cb_fun
+val cert_sign_cb:   cert_cb -> cert_sign_cb_fun 
+val cert_verify_cb: cert_cb -> cert_verify_cb_fun
+
+
+/// Defaults callbacks in configurations
+
+val defaultServerNegoCB: nego_cb 
+val defaultCertCB: cert_cb 
+
+
